\documentclass{scrartcl}
\usepackage[T1]{fontenc}
\usepackage[utf8]{inputenc}
\usepackage[ngerman]{babel}
\usepackage{amsmath,amssymb}
\usepackage{enumerate}
\usepackage{graphicx}

\newcommand{\same}{$\stackrel{\eta,\beta}{=}$}
\renewcommand{\l}{$\lambda$}

\begin{document}
\section*{Lösungen zum Lambdakalkül}
\subsection*{Aufgabe 1}
\begin{enumerate}[1.]
\item S K x y $\Rightarrow^3$ K y (x y) $\Rightarrow^2$ y und K I x y $\Rightarrow^2$ I y $\Rightarrow$ y.
\item
\begin{enumerate}[(a)]
\item (b$\to$b$\to$c)$\to$(a$\to$b)$\to$a$\to$a$\to$c
\item C I x y $\Rightarrow^3$  I y x $\Rightarrow$ y x.
\item C' f x y z = B (B C) C f x y z $\Rightarrow^3$ B C (C f) x y z \\$\Rightarrow^3$ C (C f x) y z $\Rightarrow^3$ C f x z y $\Rightarrow^3$ f z x y.
\item Mit den Ergebnissen aus (b) und (c) gilt:\\
C' (B ($\Psi$ I) (C I)) x y z $\Rightarrow^*$ B ($\Psi$ I) (C I) z x y $\Rightarrow^3$
$\Psi$ I (C I z) x y\\ $\Rightarrow^4$ I (C I z x) (C I z y) $\Rightarrow^*$ I (x z) (C I z y) $\Rightarrow^*$ I (x z) (y z) $\Rightarrow$ x z (y z).
\end{enumerate}
\end{enumerate}

\end{document}